\section{Appendices}\label{appendices}

However, the sigmoid function,
\begin{equation}
	\sigma(x) = \frac{1}{1 + e^{-x}}
	\label{eqn:sigmoid}
\end{equation}
is a special case of the generating function for the Euler polynomial coefficients,
\begin{equation}
	\frac{2e^{x t}}{1 + e^t} = \sum_{n=0}^\infty E_n(x) \frac{t^n}{n!}
\end{equation}
where, for $x = 0$,
\begin{equation}
	\sigma(x) = \frac{1}{2} \sum_{n=0}^\infty E_n(0) \frac{(-1)^n}{n!}.
	\label{eqn:sigmoid Euler expansion}
\end{equation}

The Euler polynomials at $x=0$,
\begin{equation}
	E_n(0) = -2(n+1)^{-1} \left( 2^{n+1} - 1 \right) B_{n+1}
\end{equation}
where $B_n$ is the $n^\textrm{th}$ Bernoulli number. Since Bernoulli numbers of odd index, with the exception of $B_1$, are zero, $E_i(0) = 0$ for $i = 2, 4, 6, \ldots, 2n$. Therefore, the summand and limits of Equation~(\ref{eqn:sigmoid Euler expansion}) change to
\begin{equation}
	\sigma(x) = \frac{1}{2} - \frac{1}{2} \sum_{n=1}^\infty \left( \frac{E_{2n-1(0)}}{(2n-1)!} \right) x^{2n-1}.
\end{equation}

The series representation of $E_{2n-1}(x)$
\begin{equation}
	E_{2n-1}(x) = \frac{(-1)^n 4 (2n - 1)!}{\pi^{2n+1}} \sum_{k=0}^\infty \frac{\cos [(2k + 1) \pi x]}{(2k + 1)^{2n}}
\end{equation}
such that,
\begin{equation}
	E_{2n-1}(0) = \frac{(-1)^n 4 (2n - 1)!}{\pi^{2n+1}} \sum_{k=0}^\infty \frac{1}{(2k + 1)^{2n}}
\end{equation}
and therefore,
\begin{eqnarray}
	\sigma(x) & = & \frac{1}{2} - \sum_{n=1}^\infty 2 \frac{(-1)^n}{\pi^{2n}} \left( \sum_{k=0}^\infty \frac{1}{(2k+1)^{2n}} \right) x^{2n-1} \\
		& = & \frac{1}{2} - \sum_{n=1}^\infty 2 \frac{(-1)^n}{\pi^{2n}} \left( 4^{-n} \left( 4^n - 1 \right) \zeta(2n) \right) x^{2n-1} \nonumber \\
		& = & \frac{1}{2} - \sum_{n=1}^\infty \underbrace{2 \left( \frac{-1}{4\pi^2} \right)^n \left( 4^n - 1 \right) \zeta(2n)}_{a_n} x^{2n-1} \nonumber \\
		& = & \sum_{n=0}^\infty a_n x^n,\ a_n = \left\{ \begin{array}{l l}
			1/2	& n = 0 \\
			-2 \left( \frac{-1}{4\pi^2} \right)^{(n+1)/2} \left( 4^{(n+1)/2} - 1 \right)\zeta(n+1)	& n\ \text{odd} \\
			0	& n\ \text{even}
		\end{array}\right.
		\label{eqn:sigmoid zeta expansion}
\end{eqnarray}